Obc/Fusion.v
@@ -2,7 +2,11 @@ Require Import Coq.FSets.FMapPositive.
 Require Import PArith.
 Require Import Velus.Common.
 Require Import Velus.Operators.
-Require Import Velus.Obc.
+Require Import Velus.Obc.Syntax.
+Require Import Velus.Obc.Semantics.
+Require Import Velus.Obc.Typing.
+Require Import Velus.Obc.Equiv.
+
 Require Import Velus.NLustre.Syntax.
 Require Import Velus.RMemory.
 
@@ -12,27 +16,17 @@ Open Scope list_scope.
 
 Ltac inv H := inversion H; subst; clear H.
 
-Module Type FUSEIFTE
-       (Import Ids  : IDS)
-       (Import Op   : OPERATORS)
-       (Import OpAux: OPERATORS_AUX Op)
-       (Import SynDF: Velus.NLustre.Syntax.SYNTAX Ids Op)
-       (Import SynMP: Velus.Obc.Syntax.SYNTAX Ids Op OpAux)
-       (Import SemMP: Velus.Obc.Semantics.SEMANTICS Ids Op OpAux SynMP)
-       (Import Equ  : Velus.Obc.Equiv.EQUIV Ids Op OpAux SynMP SemMP).
-
-  Inductive Is_free_in_exp : ident -> exp -> Prop :=
-  | FreeVar: forall i ty,
-      Is_free_in_exp i (Var i ty)
-  | FreeState: forall i ty,
-      Is_free_in_exp i (State i ty)
-  | FreeUnop: forall i op e ty,
-      Is_free_in_exp i e ->
-      Is_free_in_exp i (Unop op e ty)
-  |FreeBinop: forall i op e1 e2 ty,
-      Is_free_in_exp i e1 \/ Is_free_in_exp i e2 ->
-      Is_free_in_exp i (Binop op e1 e2 ty).
-
+Module Type FUSION
+       (Import Ids   : IDS)
+       (Import Op    : OPERATORS)
+       (Import OpAux : OPERATORS_AUX Op)
+       (Import SynObc: Velus.Obc.Syntax.SYNTAX Ids Op OpAux)
+       (Import SemObc: Velus.Obc.Semantics.SEMANTICS Ids Op OpAux SynObc)
+       (Import TypObc: Velus.Obc.Typing.TYPING Ids Op OpAux SynObc SemObc)
+       (Import Equ   : Velus.Obc.Equiv.EQUIV Ids Op OpAux SynObc SemObc).
+  
+  (** ** Determine whether an Obc command can modify a variable. *)
+  
   Inductive Can_write_in : ident -> stmt -> Prop :=
   | CWIAssign: forall x e,
       Can_write_in x (Assign x e)
@@ -86,87 +80,6 @@ Module Type FUSEIFTE
            | H: Can_write_in _ (Comp _ _) |- _ => inversion_clear H
            | _ => now intuition
            end.
-
-  Lemma not_free_aux1 : forall i op e ty,
-      ~Is_free_in_exp i (Unop op e ty) ->
-      ~Is_free_in_exp i e.
-  Proof.
-    intros i op e ty Hfree H; apply Hfree. now constructor. 
-  Qed.
-  
-  Lemma not_free_aux2 : forall i op e1 e2 ty,
-      ~Is_free_in_exp i (Binop op e1 e2 ty) ->
-      ~Is_free_in_exp i e1 /\ ~Is_free_in_exp i e2.
-  Proof.
-    intros i op e1 e2 ty Hfree; split; intro H; apply Hfree;
-      constructor; [now left | now right].
-  Qed.
-
-  Ltac not_free :=
-    lazymatch goal with
-    | H : ~Is_free_in_exp ?x (Var ?i ?ty) |- _ =>
-        let HH := fresh in
-        assert (HH : i <> x) by (intro; subst; apply H; constructor);
-        clear H; rename HH into H
-    | H : ~Is_free_in_exp ?x (State ?i ?ty) |- _ =>
-        let HH := fresh in
-        assert (HH : i <> x) by (intro; subst; apply H; constructor);
-        clear H; rename HH into H
-    | H : ~Is_free_in_exp ?x (Unop ?op ?e ?ty) |- _ =>
-        apply not_free_aux1 in H
-    | H : ~Is_free_in_exp ?x (Binop ?op ?e1 ?e2 ?ty) |- _ =>
-        destruct (not_free_aux2 x op e1 e2 ty H)
-    end.
-
-  (** If we add irrelevent values to [env], evaluation does not change. *)
-  Lemma exp_eval_extend_env : forall mem env x v' e v,
-      ~Is_free_in_exp x e -> exp_eval mem env e v -> exp_eval mem (PM.add x v' env) e v.
-  Proof.
-    intros mem env x v' e.
-    induction e (* using exp_ind2 *); intros v1 Hfree Heval.
-    - inv Heval. constructor. not_free. now rewrite PM.gso.
-    - inv Heval. now constructor.
-    - inv Heval. constructor.
-    - inv Heval. constructor 4 with c; trivial.
-      not_free.
-      now apply IHe.
-    - inv Heval. constructor 5 with (c1 := c1) (c2 := c2); trivial; not_free.
-      + now apply IHe1.
-      + now apply IHe2.
-  Qed.
-
-  (** If we add irrelevent values to [mem], evaluation does not change. *)
-  Lemma exp_eval_extend_mem : forall mem env x v' e v,
-      ~Is_free_in_exp x e -> exp_eval mem env e v -> exp_eval (madd_mem x v' mem) env e v.
-  Proof.
-    intros mem env x v' e.
-    induction e (* using exp_ind2 *); intros v1 Hfree Heval.
-    - inversion_clear Heval. now constructor.
-    - inversion_clear Heval. constructor. not_free. now rewrite mfind_mem_gso.
-    - inversion_clear Heval. constructor.
-    - inversion_clear Heval. constructor 4 with c; trivial.
-      not_free.
-      now apply IHe.
-    - inv Heval. constructor 5 with (c1 := c1) (c2 := c2); trivial; not_free.
-      + now apply IHe1.
-      + now apply IHe2.
-  Qed.
-
-  (** If we add objects to [mem], evaluation does not change. *)
-  Lemma exp_eval_extend_mem_by_obj : forall mem env f obj e v,
-      exp_eval mem env e v -> exp_eval (madd_obj f obj mem) env e v.
-  Proof.
-    intros mem env f v' e.
-    induction e (* using exp_ind2 *); intros v1 Heval.
-    - inversion_clear Heval. now constructor.
-    - inversion_clear Heval. constructor. now rewrite mfind_mem_add_inst.
-    - inversion_clear Heval. constructor.
-    - inversion_clear Heval. constructor 4 with c; trivial.
-      now apply IHe.
-    - inv Heval. constructor 5 with (c1 := c1) (c2 := c2); trivial.
-      + now apply IHe1.
-      + now apply IHe2.
-  Qed.
 
   Lemma cannot_write_exp_eval:
     forall prog s menv env menv' env' e v,
@@ -251,70 +164,183 @@ Module Type FUSEIFTE
         apply Iifte with (1:=Hx) (2:=Hv) (3:=Ht1).
   Qed.
 
-  Inductive IsFusible : stmt -> Prop :=
-  | IFAssign: forall x e,
-      IsFusible (Assign x e)
-  | IFAssignSt: forall x e,
-      IsFusible (AssignSt x e)
-  | IFIfte: forall e s1 s2,
-      IsFusible s1 ->
-      IsFusible s2 ->
-      (forall x, Is_free_in_exp x e -> ~Can_write_in x s1 /\ ~Can_write_in x s2) ->
-      IsFusible (Ifte e s1 s2)
-  | IFStep_ap: forall xs cls i f es,
-      IsFusible (Call xs cls i f es)
-  | IFComp: forall s1 s2,
-      IsFusible s1 ->
-      IsFusible s2 ->
-      IsFusible (Comp s1 s2)
-  | IFSkip:
-      IsFusible Skip.
+  (** ** Fusion functions *)
+  
+  Fixpoint zip s1 s2 : stmt :=
+    match s1, s2 with
+    | Ifte e1 t1 f1, Ifte e2 t2 f2 =>
+      if equiv_decb e1 e2
+      then Ifte e1 (zip t1 t2) (zip f1 f2)
+      else Comp s1 s2
+    | Skip, s => s
+    | s,    Skip => s
+    | Comp s1' s2', _ => Comp s1' (zip s2' s2)
+    | s1,   s2 => Comp s1 s2
+    end.
 
-  Lemma lift_IsFusible:
-    forall e s1 s2 t1 t2,
-      IsFusible (Comp (Ifte e s1 s2) (Ifte e t1 t2))
-      <->
-      IsFusible (Ifte e (Comp s1 t1) (Comp s2 t2)).
-  Proof.
-    Hint Constructors IsFusible.
-    intros e s1 s2 t1 t2.
-    split; intro Hifw.
-    - inversion_clear Hifw as [| | | |? ? Hs Ht|].
-      constructor; inversion_clear Hs; inversion_clear Ht; now cannot_write.
-    - inversion_clear Hifw as [| |? ? ? Hfree1 Hfree2 Hcw| | | ].
-      inversion_clear Hfree1; inversion_clear Hfree2.
-      repeat constructor; cannot_write.
-  Qed.
-
-  Lemma IsFusible_fold_left_shift:
-    forall A f (xs : list A) iacc,
-      IsFusible (fold_left (fun i x => Comp (f x) i) xs iacc)
-      <->
-      (IsFusible (fold_left (fun i x => Comp (f x) i) xs Skip)
-       /\ IsFusible iacc).
-  Proof.
-    Hint Constructors IsFusible.
-    induction xs as [|x xs IH]; [now intuition|].
-    intros; split.
-    - intro HH. simpl in HH. apply IH in HH.
-      destruct HH as [Hxs Hiacc].
-      split; [simpl; rewrite IH|];
-        repeat progress match goal with
-                        | H:IsFusible (Comp _ _) |- _ => inversion_clear H
-                        | _ => now intuition
-                        end.
-    - intros [HH0 HH1].
-      simpl in HH0; rewrite IH in HH0.
-      simpl; rewrite IH.
-      intuition.
-      repeat progress match goal with
-                      | H:IsFusible (Comp _ _) |- _ => inversion_clear H
-                      | _ => now intuition
-                      end.
-  Qed.
+  Fixpoint fuse' s1 s2 : stmt :=
+    match s1, s2 with
+    | s1, Comp s2 s3 => fuse' (zip s1 s2) s3
+    | s1, s2 => zip s1 s2
+    end.
 
   (*
-   The property "IsFusible (translate_eqns mems eqs)" is obtained above
+      NB: almost got rid of zip, but this function decreases on the first
+      argument, whereas the remaining instance of zip requires a decrease
+      on the second argument...
+
+      Fixpoint fuse' s1 s2 : stmt :=
+        match s1, s2 with
+        | Ifte e1 t1 f1, Ifte e2 t2 f2 =>
+          if exp_eqb e1 e2
+          then Ifte e1 (fuse' t1 t2) (fuse' f1 f2)
+          else Comp s1 s2
+        | s1, Comp s2 s3 => fuse' (fuse' s1 s2) s3
+        | Skip, s => s
+        | s,    Skip => s
+        | Comp s1' s2', Ifte _ _ _ => Comp s1' (zip s2' s2)
+        | s1,   s2 => Comp s1 s2
+        end.
+   *)
+
+  Definition fuse s : stmt :=
+    match s with
+    | Comp s1 s2 => fuse' s1 s2
+    | _ => s
+    end.
+
+  Definition fuse_method (m: method): method :=
+    match m with
+      mk_method name ins vars out body nodup good =>
+      mk_method name ins vars out (fuse body) nodup good
+    end.
+
+  Lemma map_m_name_fuse_methods:
+    forall methods,
+      map m_name (map fuse_method methods) = map m_name methods.
+  Proof.
+    intro ms; induction ms as [|m ms]; auto.
+    simpl. rewrite IHms.
+    now destruct m.
+  Qed.
+  
+  Program Definition fuse_class (c: class): class :=
+    match c with
+      mk_class name mems objs methods nodup nodupm =>
+      mk_class name mems objs (map fuse_method methods) nodup _
+    end.
+  Next Obligation.
+    now rewrite map_m_name_fuse_methods.
+  Qed.
+
+  (** ** Basic lemmas around [fuse_class] and [fuse_method]. *)
+
+  Lemma fuse_class_name:
+    forall c, (fuse_class c).(c_name) = c.(c_name).
+  Proof. destruct c; auto. Qed.
+
+  Lemma fuse_method_name:
+    forall m, (fuse_method m).(m_name) = m.(m_name).
+  Proof. destruct m; auto. Qed.
+
+  Lemma fuse_method_in:
+    forall m, (fuse_method m).(m_in) = m.(m_in). 
+  Proof. destruct m; auto. Qed.
+
+  Lemma fuse_method_out:
+    forall m, (fuse_method m).(m_out) = m.(m_out). 
+  Proof. destruct m; auto. Qed.
+
+  Lemma fuse_find_class:
+    forall p id c p',
+      find_class id p = Some (c, p') ->
+      find_class id (map fuse_class p) = Some (fuse_class c, map fuse_class p').
+  Proof.
+    induction p as [|c']; simpl; intros ** Find; try discriminate.
+    rewrite fuse_class_name.
+    destruct (ident_eqb (c_name c') id); auto.
+    inv Find; auto.
+  Qed.
+
+  Lemma fuse_find_method:
+    forall id c m,
+      find_method id (fuse_class c).(c_methods) = Some m ->
+      exists m', m = fuse_method m'
+                 /\ find_method id c.(c_methods) = Some m'.
+  Proof.
+    intros ** Find.
+    destruct c as [? ? ? meths ? Nodup]; simpl in *.
+    induction meths as [|m']; simpl in *; try discriminate.
+    inv Nodup; auto.
+    rewrite fuse_method_name in Find.
+    destruct (ident_eqb (m_name m') id); auto.
+    inv Find.
+    exists m'; auto.
+  Qed.
+
+  Lemma fuse_class_c_objs:
+    forall c,
+      (fuse_class c).(c_objs) = c.(c_objs).
+  Proof.
+    unfold fuse_class. destruct c; auto.
+  Qed.
+
+  Lemma fuse_class_c_mems:
+    forall c,
+      (fuse_class c).(c_mems) = c.(c_mems).
+  Proof.
+    unfold fuse_class. destruct c; auto.
+  Qed.
+
+  Lemma fuse_class_c_name:
+    forall c,
+      (fuse_class c).(c_name) = c.(c_name).
+  Proof.
+    unfold fuse_class. destruct c; auto.
+  Qed.
+
+  Lemma fuse_method_m_name:
+    forall m,
+      (fuse_method m).(m_name) = m.(m_name).
+  Proof.
+    unfold fuse_method; destruct m; auto.
+  Qed.
+
+  Lemma fuse_method_body:
+    forall fm,
+      (fuse_method fm).(m_body) = fuse fm.(m_body).
+  Proof.
+    now destruct fm.
+  Qed.
+
+  Lemma map_fuse_class_c_name:
+    forall p,
+      map (fun cls => (fuse_class cls).(c_name)) p = map c_name p.
+  Proof.
+    induction p; auto.
+    simpl. now rewrite IHp, fuse_class_c_name.
+  Qed.
+
+  Lemma fuse_find_method':
+    forall f fm cls,
+      find_method f cls.(c_methods) = Some fm ->
+      find_method f (fuse_class cls).(c_methods) = Some (fuse_method fm).
+  Proof.
+    destruct cls; simpl.
+    induction c_methods0 as [|m ms]; inversion 1.
+    simpl.
+    destruct (ident_eq_dec m.(m_name) f) as [He|Hne].
+    - rewrite fuse_method_m_name, He, ident_eqb_refl in *.
+      now injection H1; intro; subst.
+    - apply ident_eqb_neq in Hne.
+      rewrite fuse_method_m_name, Hne in *.
+      inv c_nodupm0; auto.
+  Qed.
+  
+  (** ** Invariant sufficient to justify semantic preservation of fusion. *)
+  
+  (*
+   The property "Fusible (translate_eqns mems eqs)" is obtained above
    using scheduling assumptions for EqDef, since they are needed to treat
    the translation of merge expressions, and clocking assumptions for EqApp and
    EqFby. While the EqApp case can also be obtained from the scheduling
@@ -330,7 +356,7 @@ Module Type FUSEIFTE
       if x { mem(x) = y }
 
    This program is well scheduled, but it does not satisfy the invariant
-   IsFusible. We could imagine a weaker invariant that allows the
+   Fusible. We could imagine a weaker invariant that allows the
    right-most write under an expression to change free variables in the
    expression, which suffices to justify the optimisation, but the
    preservation of this invariant under the optimisation likely becomes much
@@ -343,17 +369,70 @@ Module Type FUSEIFTE
    are effectively always present).
   *)
 
-  Fixpoint zip s1 s2 : stmt :=
-    match s1, s2 with
-    | Ifte e1 t1 f1, Ifte e2 t2 f2 =>
-      if equiv_decb e1 e2
-      then Ifte e1 (zip t1 t2) (zip f1 f2)
-      else Comp s1 s2
-    | Skip, s => s
-    | s,    Skip => s
-    | Comp s1' s2', _ => Comp s1' (zip s2' s2)
-    | s1,   s2 => Comp s1 s2
-    end.
+  Inductive Fusible : stmt -> Prop :=
+  | IFAssign: forall x e,
+      Fusible (Assign x e)
+  | IFAssignSt: forall x e,
+      Fusible (AssignSt x e)
+  | IFIfte: forall e s1 s2,
+      Fusible s1 ->
+      Fusible s2 ->
+      (forall x, Is_free_in_exp x e -> ~Can_write_in x s1 /\ ~Can_write_in x s2) ->
+      Fusible (Ifte e s1 s2)
+  | IFStep_ap: forall xs cls i f es,
+      Fusible (Call xs cls i f es)
+  | IFComp: forall s1 s2,
+      Fusible s1 ->
+      Fusible s2 ->
+      Fusible (Comp s1 s2)
+  | IFSkip:
+      Fusible Skip.
+
+  Definition ClassFusible (c: class) : Prop :=
+    Forall (fun m=> Fusible m.(m_body)) c.(c_methods).
+
+  Lemma lift_Fusible:
+    forall e s1 s2 t1 t2,
+      Fusible (Comp (Ifte e s1 s2) (Ifte e t1 t2))
+      <->
+      Fusible (Ifte e (Comp s1 t1) (Comp s2 t2)).
+  Proof.
+    Hint Constructors Fusible.
+    intros e s1 s2 t1 t2.
+    split; intro Hifw.
+    - inversion_clear Hifw as [| | | |? ? Hs Ht|].
+      constructor; inversion_clear Hs; inversion_clear Ht; now cannot_write.
+    - inversion_clear Hifw as [| |? ? ? Hfree1 Hfree2 Hcw| | | ].
+      inversion_clear Hfree1; inversion_clear Hfree2.
+      repeat constructor; cannot_write.
+  Qed.
+
+  Lemma Fusible_fold_left_shift:
+    forall A f (xs : list A) iacc,
+      Fusible (fold_left (fun i x => Comp (f x) i) xs iacc)
+      <->
+      (Fusible (fold_left (fun i x => Comp (f x) i) xs Skip)
+       /\ Fusible iacc).
+  Proof.
+    Hint Constructors Fusible.
+    induction xs as [|x xs IH]; [now intuition|].
+    intros; split.
+    - intro HH. simpl in HH. apply IH in HH.
+      destruct HH as [Hxs Hiacc].
+      split; [simpl; rewrite IH|];
+        repeat progress match goal with
+                        | H:Fusible (Comp _ _) |- _ => inversion_clear H
+                        | _ => now intuition
+                        end.
+    - intros [HH0 HH1].
+      simpl in HH0; rewrite IH in HH0.
+      simpl; rewrite IH.
+      intuition.
+      repeat progress match goal with
+                      | H:Fusible (Comp _ _) |- _ => inversion_clear H
+                      | _ => now intuition
+                      end.
+  Qed.
 
   Lemma Can_write_in_zip:
     forall s1 s2 x,
@@ -394,11 +473,11 @@ Module Type FUSEIFTE
   
   Lemma zip_free_write:
     forall s1 s2,
-      IsFusible s1
-      -> IsFusible s2
-      -> IsFusible (zip s1 s2).
+      Fusible s1
+      -> Fusible s2
+      -> Fusible (zip s1 s2).
   Proof.
-    Hint Constructors IsFusible Can_write_in.
+    Hint Constructors Fusible Can_write_in.
     induction s1, s2;
       intros Hfree1 Hfree2;
       inversion_clear Hfree1;
@@ -413,10 +492,10 @@ Module Type FUSEIFTE
       constructor;
       repeat progress
              match goal with
-             | H1:IsFusible ?s1,
-                 H2:IsFusible ?s2,
-                 Hi:context [IsFusible (zip _ _)]
-               |- IsFusible (zip ?s1 ?s2)
+             | H1:Fusible ?s1,
+                 H2:Fusible ?s2,
+                 Hi:context [Fusible (zip _ _)]
+               |- Fusible (zip ?s1 ?s2)
                => apply Hi with (1:=H1) (2:=H2)
              | |- forall x, Is_free_in_exp x ?e -> _
                => intros x Hfree
@@ -432,7 +511,7 @@ Module Type FUSEIFTE
   
   Lemma zip_Comp':
     forall s1 s2,
-      IsFusible s1
+      Fusible s1
       -> (stmt_eval_eq (zip s1 s2) (Comp s1 s2)).
   Proof.
     induction s1, s2;
@@ -447,7 +526,7 @@ Module Type FUSEIFTE
                => destruct (equiv_decb e1 e2) eqn:Heq;
                     (rewrite equiv_decb_equiv in Heq; rewrite <-Heq in *)
                     || rewrite not_equiv_decb_equiv in Heq 
-             | H:IsFusible ?s1,
+             | H:Fusible ?s1,
                  IH:context [stmt_eval_eq (zip ?s1 _) _]
                |- context [zip ?s1 ?s2]
                => rewrite IH with (1:=H)
@@ -457,42 +536,11 @@ Module Type FUSEIFTE
       reflexivity.
   Qed.
   
-  Fixpoint fuse' s1 s2 : stmt :=
-    match s1, s2 with
-    | s1, Comp s2 s3 => fuse' (zip s1 s2) s3
-    | s1, s2 => zip s1 s2
-    end.
-
-  (*
-      NB: almost got rid of zip, but this function decreases on the first
-      argument, whereas the remaining instance of zip requires a decrease
-      on the second argument...
-
-      Fixpoint fuse' s1 s2 : stmt :=
-        match s1, s2 with
-        | Ifte e1 t1 f1, Ifte e2 t2 f2 =>
-          if exp_eqb e1 e2
-          then Ifte e1 (fuse' t1 t2) (fuse' f1 f2)
-          else Comp s1 s2
-        | s1, Comp s2 s3 => fuse' (fuse' s1 s2) s3
-        | Skip, s => s
-        | s,    Skip => s
-        | Comp s1' s2', Ifte _ _ _ => Comp s1' (zip s2' s2)
-        | s1,   s2 => Comp s1 s2
-        end.
-   *)
-
-  Definition fuse s : stmt :=
-    match s with
-    | Comp s1 s2 => fuse' s1 s2
-    | _ => s
-    end.
-
   Lemma fuse'_free_write:
     forall s2 s1,
-      IsFusible s1
-      -> IsFusible s2
-      -> IsFusible (fuse' s1 s2).
+      Fusible s1
+      -> Fusible s2
+      -> Fusible (fuse' s1 s2).
   Proof.
     induction s2;
       try (intros; apply zip_free_write; assumption).
@@ -509,7 +557,7 @@ Module Type FUSEIFTE
   Require Import Setoid.
   
   Definition fuse_eval_eq s1 s2: Prop :=
-    stmt_eval_eq s1 s2 /\ (IsFusible s1 /\ IsFusible s2).
+    stmt_eval_eq s1 s2 /\ (Fusible s1 /\ Fusible s2).
   
   (*
      Print relation.
@@ -518,7 +566,7 @@ Module Type FUSEIFTE
 
   Lemma fuse_eval_eq_refl:
     forall s,
-      IsFusible s
+      Fusible s
       -> Proper fuse_eval_eq s.
   Proof.
     intros s Hfree; unfold Proper, fuse_eval_eq; intuition.
@@ -559,8 +607,8 @@ Module Type FUSEIFTE
   
   Lemma zip_Comp:
     forall s1 s2,
-      IsFusible s1
-      -> IsFusible s2
+      Fusible s1
+      -> Fusible s2
       -> fuse_eval_eq (zip s1 s2) (Comp s1 s2).
   Proof.
     intros s1 s2 Hfree1 Hfree2.
@@ -585,7 +633,7 @@ Module Type FUSEIFTE
   Instance fuse_eval_eq_Comp_Proper:
     Proper (fuse_eval_eq ==> fuse_eval_eq ==> fuse_eval_eq) Comp.
   Proof.
-    Hint Constructors IsFusible.
+    Hint Constructors Fusible.
     intros s s' Hseq t t' Hteq.
     unfold fuse_eval_eq in *.
     destruct Hseq as [Hseq [Hfrees Hfrees']].
@@ -610,11 +658,11 @@ Module Type FUSEIFTE
   
   Lemma fuse'_Comp:
     forall s2 s1,
-      IsFusible s1
-      -> IsFusible s2
+      Fusible s1
+      -> Fusible s2
       -> stmt_eval_eq (fuse' s1 s2) (Comp s1 s2).
   Proof.
-    Hint Constructors IsFusible.
+    Hint Constructors Fusible.
     induction s2;
       intros s1 Hifte1 Hifte2; simpl;
         try now (rewrite zip_Comp'; intuition).
@@ -622,11 +670,11 @@ Module Type FUSEIFTE
     inversion_clear Hifte2.
     rewrite IHs2_2;
       match goal with
-      | H1:IsFusible ?s1,
-      H2:IsFusible ?s2 |- IsFusible (zip ?s1 ?s2)
+      | H1:Fusible ?s1,
+      H2:Fusible ?s2 |- Fusible (zip ?s1 ?s2)
         => apply zip_free_write with (1:=H1) (2:=H2)
-      | |- IsFusible ?s => assumption
-      | H:IsFusible s2_2 |- _ => pose proof (fuse_eval_eq_refl _ H)
+      | |- Fusible ?s => assumption
+      | H:Fusible s2_2 |- _ => pose proof (fuse_eval_eq_refl _ H)
       end.
     intros prog menv env menv' env'.
     rewrite zip_Comp; [now apply iff_refl|assumption|assumption].
@@ -648,7 +696,7 @@ Module Type FUSEIFTE
 
   Lemma fuse_Comp:
     forall s,
-      IsFusible s
+      Fusible s
       -> stmt_eval_eq (fuse s) s.
   Proof.
     intros s Hfree prog menv env menv' env'.
@@ -656,24 +704,178 @@ Module Type FUSEIFTE
     inversion_clear Hfree.
     destruct s2;
       match goal with
-      | H: IsFusible ?s2 |- context [fuse' _ ?s2]
+      | H: Fusible ?s2 |- context [fuse' _ ?s2]
         => pose proof (fuse_eval_eq_refl _ H)
       end;
       rewrite fuse'_Comp; auto; reflexivity.
   Qed.
 
-End FUSEIFTE.
+  Lemma fuse_call:
+    forall p n me me' f xss rs,
+      Forall ClassFusible p ->
+      stmt_call_eval p me n f xss me' rs ->
+      stmt_call_eval (map fuse_class p) me n f xss me' rs.
+  Proof.
+    cut ((forall p me ve stmt e',
+             stmt_eval p me ve stmt e' ->
+             Forall ClassFusible p ->
+             stmt_eval (map fuse_class p) me ve stmt e')
+         /\ (forall p me clsid f vs me' rvs,
+                stmt_call_eval p me clsid f vs me' rvs ->
+                Forall ClassFusible p ->
+                stmt_call_eval (map fuse_class p) me clsid f vs me' rvs)).
+    now destruct 1 as (Hf1 & Hf2); intros; apply Hf2; auto.
+    apply stmt_eval_call_ind; intros; eauto using stmt_eval.
+    pose proof (find_class_In _ _ _ _ H) as Hinp.
+    pose proof (find_method_In _ _ _ H0) as Hinc.
+    pose proof (find_class_app _ _ _ _ H) as Hprog'.
+    apply fuse_find_class in H.
+    apply fuse_find_method' in H0.
+    econstructor; eauto.
+    2:now rewrite fuse_method_out; eassumption.
+    rewrite fuse_method_in.
+    apply In_Forall with (1:=H4) in Hinp.
+    apply In_Forall with (1:=Hinp) in Hinc.
+    rewrite fuse_method_body.
+    rewrite fuse_Comp with (1:=Hinc).
+    apply H2.
+    destruct Hprog' as (cls'' & Hprog & Hfind).
+    rewrite Hprog in H4.
+    apply Forall_app in H4.
+    rewrite Forall_cons2 in H4.
+    intuition.
+  Qed.
 
-Module FuseIfteFun
+  (** ** Fusion preserves well-typing. *)
+
+  Lemma wt_stmt_map_fuse_class:
+    forall p objs mems vars body,
+      wt_stmt p objs mems vars body ->
+      wt_stmt (map fuse_class p) objs mems vars body.
+  Proof.
+    induction body; inversion_clear 1; eauto using wt_stmt.
+    eapply wt_Call
+    with (cls:=fuse_class cls) (p':=map fuse_class p') (fm:=fuse_method fm);
+      auto; try (now destruct fm; auto).
+    erewrite fuse_find_class; eauto.
+    now apply fuse_find_method'.
+  Qed.
+
+  Lemma wt_stmt_zip:
+    forall p objs mems vars s1 s2,
+      wt_stmt p objs mems vars s1 ->
+      wt_stmt p objs mems vars s2 ->
+      wt_stmt p objs mems vars (zip s1 s2).
+  Proof.
+    induction s1, s2; simpl; repeat inversion_clear 1; eauto using wt_stmt.
+    destruct (exp_dec e e0) as [He|Hne].
+    - rewrite He, equiv_decb_refl; eauto using wt_stmt.
+    - apply not_equiv_decb_equiv in Hne. rewrite Hne. eauto using wt_stmt.
+  Qed.
+
+  Lemma zip_wt:
+    forall p insts mems vars s1 s2,
+      wt_stmt p insts mems vars s1 ->
+      wt_stmt p insts mems vars s2 ->
+      wt_stmt p insts mems vars (zip s1 s2).
+  Proof.
+    induction s1, s2; simpl;
+      try match goal with |- context [if ?e1 ==b ?e2 then _ else _] =>
+                          destruct (equiv_decb e1 e2) end;
+      auto with obctyping;
+      inversion_clear 1;
+      try inversion_clear 2;
+      auto with obctyping.
+    inversion_clear 1.
+    auto with obctyping.
+  Qed.
+
+  Lemma fuse_wt:
+    forall p insts mems vars s,
+      wt_stmt p insts mems vars s ->
+      wt_stmt p insts mems vars (fuse s).
+  Proof.
+    intros ** WTs.
+    destruct s; auto; simpl; inv WTs.
+    match goal with H1:wt_stmt _ _ _ _ s1, H2:wt_stmt _ _ _ _ s2 |- _ =>
+                    revert s2 s1 H1 H2 end.
+    induction s2; simpl; auto using zip_wt.
+    intros s2 WTs1 WTcomp.
+    inv WTcomp.
+    apply IHs2_2; auto.
+    apply zip_wt; auto.
+  Qed.
+
+  Lemma fuse_wt_program:
+    forall G,
+      wt_program G ->
+      wt_program (map fuse_class G).
+  Proof.
+    intros ** WTG.
+    induction G as [|c p]; simpl;
+      inversion_clear WTG as [|? ? Wtc Wtp Nodup]; constructor; auto.
+    - inversion_clear Wtc as (Hos & Hms).
+      constructor.
+      + rewrite fuse_class_c_objs.
+        apply Forall_impl_In with (2:=Hos).
+        intros ic Hin Hfind.
+        apply not_None_is_Some in Hfind.
+        destruct Hfind as ((cls & p') & Hfind).
+        rewrite fuse_find_class with (1:=Hfind).
+        discriminate.
+      + destruct c; simpl in *.
+        clear Nodup c_nodup0 c_nodupm0 Hos IHp Wtp.
+        induction c_methods0 as [|m ms]; simpl; auto using Forall_nil.
+        apply Forall_cons2 in Hms.
+        destruct Hms as (WTm & WTms).
+        apply Forall_cons; auto. clear IHms WTms.
+        unfold wt_method in *.
+        destruct m; unfold meth_vars in *; simpl in *.
+        clear m_nodupvars0 m_good0.
+        apply wt_stmt_map_fuse_class.
+        destruct m_body0; simpl; inv WTm; eauto using wt_stmt.
+        revert m_body0_1 H1.
+        induction m_body0_2; simpl; eauto using wt_stmt_zip.
+        intros s1 WT1. inv H2.
+        eauto using wt_stmt_zip.
+    - simpl.
+      now rewrite fuse_class_c_name, map_map, map_fuse_class_c_name.
+  Qed.
+
+  Lemma fuse_wt_mem:
+    forall me p c,
+      wt_mem me p c ->
+      wt_mem me (map fuse_class p) (fuse_class c).
+  Proof.
+    intros ** Hwt_mem.
+    induction Hwt_mem
+              using wt_mem_ind_mult
+    with (P := fun me p cl Hwt => wt_mem me (map fuse_class p) (fuse_class cl))
+         (Pinst := fun me p oc Hwt_inst => wt_mem_inst me (map fuse_class p) oc).
+    - constructor.
+      + rewrite fuse_class_c_mems; auto.
+      + rewrite fuse_class_c_objs.
+        eapply Forall_forall; intros oc Hin.
+        eapply In_Forall in H as [? ?]; eauto.
+    - now constructor.
+    - simpl in *.
+      econstructor 2; eauto.
+      apply fuse_find_class. eauto.
+  Qed.
+  
+End FUSION.
+
+Module FusionFun
        (Import Ids  : IDS)
        (Import Op   : OPERATORS)
        (Import OpAux: OPERATORS_AUX Op)
-       (Import SynDF: Velus.NLustre.Syntax.SYNTAX Ids Op)
-       (Import SynMP: Velus.Obc.Syntax.SYNTAX Ids Op OpAux)
-       (Import SemMP: Velus.Obc.Semantics.SEMANTICS Ids Op OpAux SynMP)
-       (Import Equ  : Velus.Obc.Equiv.EQUIV Ids Op OpAux SynMP SemMP)
-       <: FUSEIFTE Ids Op OpAux SynDF SynMP SemMP Equ.
+       (Import SynObc: Velus.Obc.Syntax.SYNTAX Ids Op OpAux)
+       (Import SemObc: Velus.Obc.Semantics.SEMANTICS Ids Op OpAux SynObc)
+       (Import TypObc: Velus.Obc.Typing.TYPING Ids Op OpAux SynObc SemObc)
+       (Import Equ  : Velus.Obc.Equiv.EQUIV Ids Op OpAux SynObc SemObc)
+       <: FUSION Ids Op OpAux SynObc SemObc TypObc Equ.
 
-  Include FUSEIFTE Ids Op OpAux SynDF SynMP SemMP Equ.
+  Include FUSION Ids Op OpAux SynObc SemObc TypObc Equ.
 
-End FuseIfteFun.
+End FusionFun.
+
