Instantiator.v
@@ -11,21 +11,21 @@ Require Import NLustreToObc.Correctness.MemoryCorres.
 Require Import NLustre.
 Require Import Obc.
 Require Import NLustreToObc.Translation.
+Require Import NLustreToObc.Fusible.
 Require Import NLustre.Memories.
-Require Import Obc.FuseIfte.
 Require Import NLustre.IsFree.Decide.
 Require Import NLustre.WellFormed.Decide.
 Require Import NLustre.Typing.
 
-Module DF := NLustreFun Ids Op OpAux.
+Module NL := NLustreFun Ids Op OpAux.
 Module Obc := ObcFun Ids Op OpAux.
-Module Mem := MemoriesFun Ids Op DF.Syn.
-Module Trans := TranslationFun Ids Op OpAux DF.Syn Obc.Syn Mem.
-Module IsP := IsPresentFun Ids Op OpAux DF.Syn Obc.Syn Obc.Sem Mem Trans.
-Module MemCor := MemoryCorresFun Ids Op OpAux DF Obc.
-Module Fus := FuseIfteFun Ids Op OpAux DF.Syn Obc.Syn Obc.Sem Obc.Equ.
-Module Typ := NLustreToObc.Typing.TypingFun Ids Op OpAux DF Obc Mem Trans Fus.
-Module Corr := NLustreToObc.Correctness.CorrectnessFun Ids Op OpAux DF Obc Mem Trans IsP MemCor Fus Typ.
+Module Mem := MemoriesFun Ids Op NL.Syn.
+Module Trans := TranslationFun Ids Op OpAux NL.Syn Obc.Syn Mem.
+Module IsP := IsPresentFun Ids Op OpAux NL.Syn Obc.Syn Obc.Sem Mem Trans.
+Module MemCor := MemoryCorresFun Ids Op OpAux NL Obc.
+Module Typ := NLustreToObc.Typing.TypingFun Ids Op OpAux NL Obc Mem Trans.
+Module Corr := NLustreToObc.Correctness.CorrectnessFun Ids Op OpAux NL Obc Mem Trans IsP MemCor Typ.
+Module Fusible := NLustreToObc.Fusible.FusibleFun Ids Op OpAux NL Obc Trans.
 
-  
-Module WeFDec := WellFormed.Decide.Decide Ids Op DF.Syn DF.IsF DF.IsFDec DF.Ord DF.Mem DF.IsD DF.IsV DF.IsDDec DF.IsVDec DF.NoD DF.WeF.
+Module WeFDec := WellFormed.Decide.Decide Ids Op NL.Syn NL.IsF NL.IsFDec NL.Ord NL.Mem NL.IsD NL.IsV NL.IsDDec NL.IsVDec NL.NoD NL.WeF.
+
