NLustreToObc/Typing.v
@@ -10,7 +10,6 @@ Require Import Velus.RMemory.
 Require Import Velus.NLustre.
 Require Import Velus.Obc.
 Require Import Velus.NLustreToObc.Translation.
-Require Import Velus.Obc.FuseIfte.
 
 Require Import Velus.NLustre.Typing.
 
@@ -24,47 +23,10 @@ Module Type TYPING
        (Import Obc   : OBC Ids Op OpAux)
        (Import Mem   : MEMORIES Ids Op DF.Syn)
 
-       (Import Trans : TRANSLATION Ids Op OpAux DF.Syn Obc.Syn Mem)
-
-       (Import Fus   : FUSEIFTE Ids Op OpAux DF.Syn Obc.Syn Obc.Sem Obc.Equ).
+       (Import Trans : TRANSLATION Ids Op OpAux DF.Syn Obc.Syn Mem).
 
 
   (** Preservation of well-typing. *)
-
-  (** For the ifte fusion optimization *)
-
-  Lemma zip_wt:
-    forall p insts mems vars s1 s2,
-      wt_stmt p insts mems vars s1 ->
-      wt_stmt p insts mems vars s2 ->
-      wt_stmt p insts mems vars (zip s1 s2).
-  Proof.
-    induction s1, s2; simpl;
-      try match goal with |- context [if ?e1 ==b ?e2 then _ else _] =>
-            destruct (equiv_decb e1 e2) end;
-      auto with obctyping;
-      inversion_clear 1;
-      try inversion_clear 2;
-      auto with obctyping.
-    inversion_clear 1.
-    auto with obctyping.
-  Qed.
-
-  Lemma fuse_wt:
-    forall p insts mems vars s,
-      wt_stmt p insts mems vars s ->
-      wt_stmt p insts mems vars (fuse s).
-  Proof.
-    intros ** WTs.
-    destruct s; auto; simpl; inv WTs.
-    match goal with H1:wt_stmt _ _ _ _ s1, H2:wt_stmt _ _ _ _ s2 |- _ =>
-                    revert s2 s1 H1 H2 end.
-    induction s2; simpl; auto using zip_wt.
-    intros s2 WTs1 WTcomp.
-    inv WTcomp.
-    apply IHs2_2; auto.
-    apply zip_wt; auto.
-  Qed.
 
   Section Expressions.
 
@@ -561,11 +523,8 @@ Module TypingFun
        (Import DF    : NLUSTRE Ids Op OpAux)
        (Import Obc   : OBC Ids Op OpAux)
        (Import Mem   : MEMORIES Ids Op DF.Syn)
-
        (Import Trans : TRANSLATION Ids Op OpAux DF.Syn Obc.Syn Mem)
+       <: TYPING Ids Op OpAux DF Obc Mem Trans.
 
-       (Import Fus   : FUSEIFTE Ids Op OpAux DF.Syn Obc.Syn Obc.Sem Obc.Equ)
-       <: TYPING Ids Op OpAux DF Obc Mem Trans Fus.
-
-       Include TYPING Ids Op OpAux DF Obc Mem Trans Fus.
+       Include TYPING Ids Op OpAux DF Obc Mem Trans.
 End TypingFun.    
